Turing Reducciones/Envasado.dfy
@@ -1,4 +1,4 @@
-include "../Especificaciones/Envasado.dfy"
+include "../Especificaciones/EnvasadoOpt.dfy"
 
 lemma treductionPOE_to_PDE(A : multiset<nat>, E : nat, I:multiset<multiset<nat>>)
     ensures forall k : nat | k >= |I| :: optimalEnvasado(A, E, I) ==> Envasar(A, E, k)
