Turing Reducciones/VertexCoverTRed.dfy
@@ -1,0 +1,19 @@
+include "../Especificaciones/VertexCoverOpt.dfy"
+
+lemma treductionPCVO_to_PDCV(graph : Graph, I : set<Node>)
+    requires isValidGraph(graph) 
+    ensures forall k | k >= |I| :: optimalVertexCover(graph, I) ==> VertexCover(graph, k)
+    ensures forall k | k < |I| :: optimalVertexCover(graph, I) ==> !VertexCover(graph, k)
+{}
+
+method {:axiom} mVertexCover (graph:Graph, k:int, I:set<Node>) returns (b:bool)
+  requires isValidGraph(graph)
+  ensures b == (I <= graph.0 && |I| >= k && isVertexCover(I,graph))
+
+method {:axiom} moptimalValueVertexCover (graph:Graph) returns (k:nat) //Tipo nat comentar
+  requires isValidGraph(graph)
+  ensures optimalValueVertexCover(graph,k)
+
+method {:axiom} moptimalVertexCover (graph : Graph) returns (I:set<Node>)
+  requires isValidGraph(graph)
+  ensures optimalVertexCover(graph,I)
